Verifications so far. SubNode, NotNode and OrNode complete

Optimizations/Canonicalizations/Common.thy
@@ -6,6 +6,22 @@ theory Common
     Semantics.IRTreeEvalThms
 begin
 
+
+(* Old size function
+fun size :: "IRExpr \<Rightarrow> nat" where
+  (* "size (UnaryExpr op e) = (size e) + 1" | *) (* Old, new below. *)
+  "size (UnaryExpr op e) = (size e) * 2" |
+  "size (BinaryExpr op x y) = (size x) + ((size y) * 2)" |
+ (* "size (BinaryExpr op x y) = (size x) + (size y)" |*)
+  "size (ConditionalExpr cond t f) = (size cond) + (size t) + (size f) + 2" |
+  "size (ConstantExpr c) = 1" |
+  "size (ParameterExpr ind s) = 2" |
+  "size (LeafExpr nid s) = 2" |
+  "size (ConstantVar c) = 2" |
+  "size (VariableExpr x s) = 2"
+*)
+
+
 lemma size_pos[simp]: "0 < size y"
   apply (induction y; auto?)
   subgoal premises prems for op a b
