Optimizations/Canonicalizations/AddPhase.thy
@@ -269,11 +269,71 @@ lemma AddToSubHelperLowLevel:
 
 optimization AddToSub: "-e + y \<longmapsto> y - e"
   using AddToSubHelperLowLevel by auto
-  end
+  
 
 print_phases
 
 
+(* -----  Starts here -----  *)
+
+(* 
+ AddNode has 8 optimisations total
+ Currently *6* optimisations are verified.
+
+ -- Already verified above --
+
+ - AddShiftRightConst
+ - RedundantSubAdd
+ - AddNeutral (32-bit only)
+
+ -- Verified below --
+ 
+ - RedundantAddSub
+ - AddRightNegateToSub
+ - AddLeftNegateToSub 
+
+*)
+
+(* Value level proofs *)
+lemma val_redundant_add_sub:
+  assumes "b \<noteq> UndefVal \<and> a \<noteq> UndefVal \<and> intval_add b a \<noteq> UndefVal"
+  shows "val[(b + a) - b] = val[a]"
+  using assms apply (cases a; cases b; auto)
+  done
+
+lemma val_add_right_negate_to_sub:
+  assumes "x \<noteq> UndefVal \<and> e \<noteq> UndefVal \<and> intval_add x e \<noteq> UndefVal"
+  shows "val[x + (-e)] = val[x - e]"
+  using assms apply (cases x; cases e; auto)
+  done
+
+(* Exp level proofs *)
+lemma exp_add_left_negate_to_sub:
+ "exp[-e + y] \<ge> exp[y - e]"
+  apply (cases e; cases y; auto)
+  using AddToSubHelperLowLevel apply auto+
+  done
+
+(* Optimizations *)
+optimization opt_redundant_sub_add: "(b + a) - b \<longmapsto> a"
+   apply unfold_optimization apply simp_all apply auto using val_redundant_add_sub 
+   apply (metis evalDet intval_add.simps(10) intval_sub.simps(10))
+  done
+
+optimization opt_add_right_negate_to_sub: "(x + (-e)) \<longmapsto> x - e"
+   apply unfold_optimization apply simp_all apply auto using AddToSubHelperLowLevel intval_add_sym 
+   apply auto
+  done
+
+optimization opt_add_left_negate_to_sub: "-x + y \<longmapsto> y - x"
+  using exp_add_left_negate_to_sub rewrite_preservation.simps(1) apply blast apply simp_all
+  done
+  
+
+
+(* ----- Ends here ----- *)
+
+end
 
 
 
