Optimizations/Canonicalizations/MulPhase.thy
@@ -1,0 +1,157 @@
+theory MulPhase
+  imports
+    Common
+begin
+
+section \<open>Optimizations for Mul Nodes\<close>
+
+phase MulPhase
+  terminating size
+begin
+
+(* Word level proofs *)
+lemma bin_eliminate_redundant_negative:
+ "uminus (x :: 'a::len word) * uminus (y :: 'a::len word) = x * y"
+  by simp
+
+lemma bin_multiply_neutral:
+ "(x :: 'a::len word) * 1 = x"
+  by simp
+
+lemma bin_multiply_zero:
+ "(x :: 'a::len word) * 0 = 0"
+  by simp
+
+lemma bin_multiply_negative:
+ "(x :: 'a::len word) * uminus 1 = uminus x"
+  by simp
+
+lemma bin_multiply_power_2:
+ "(x:: 'a::len word) * (2^j) = x << j"
+  by simp
+
+(* Value level proofs *)
+lemma val_eliminate_redundant_negative:
+  assumes "x \<noteq> UndefVal \<and> y \<noteq> UndefVal \<and> (intval_negate x * intval_negate y) \<noteq> UndefVal"
+  shows "intval_mul val[-x] val[-y] = intval_mul x y"
+  apply (cases x; cases y; auto)
+  done
+
+lemma val_multiply_neutral_32:
+  assumes "is_IntVal32 x"
+  shows "val[x] *  (IntVal32 1) = val[x]"
+  using assms is_IntVal32_def times_Value_def by fastforce
+
+lemma val_multiply_neutral_64:
+  assumes "is_IntVal64 x"
+  shows "val[x] *  (IntVal64 1) = val[x]"
+  using assms 
+   apply (metis Value.collapse(2) intval_mul.simps(2) mult.right_neutral times_Value_def)
+  done
+
+lemma val_multiply_zero_32:
+  assumes "is_IntVal32 x"
+  shows "val[x] * (IntVal32 0) = IntVal32 0"
+  using assms 
+  by (metis Value.collapse(1) intval_mul.simps(1) mult_not_zero times_Value_def)
+
+lemma val_multiply_zero_64:
+  assumes "is_IntVal64 x"
+  shows "val[x] * (IntVal64 0) = IntVal64 0"
+   using assms intval_mul.simps(2) 
+  by (metis Value.collapse(2) mult_zero_right times_Value_def)
+
+lemma val_multiply_negative_32:
+  assumes "is_IntVal32 x"
+  shows "x * intval_negate (IntVal32 1) = intval_negate x"
+  using assms is_IntVal32_def times_Value_def by force
+
+lemma val_multiply_negative_64:
+  assumes "is_IntVal64 x"
+  shows "x * intval_negate (IntVal64 1) = intval_negate x"
+  using assms is_IntVal64_def times_Value_def by fastforce
+
+
+lemma val_multiply_power_2:
+  fixes j :: "32 word"
+  assumes "is_IntVal32 x \<and> j \<ge> 0 \<and> j_AsNat = (nat (Values.intval (IntVal32 j)))"
+  shows "x * IntVal32 (2 ^ j_AsNat) = intval_left_shift x (IntVal32 j)"
+  using assms apply (cases x; cases j; cases j_AsNat; auto)
+  sorry
+
+
+(* Exp-level proofs *)
+
+lemma exp_multiply_zero_64:
+ "BinaryExpr BinMul x (ConstantExpr (IntVal64 0)) \<ge> ConstantExpr (IntVal64 0)"
+   apply (cases x; auto) using val_multiply_zero_64 unfold_const64 
+   apply (metis intval_mul.simps(12) is_IntVal32_def is_IntVal_def times_Value_def unary_eval_int)
+          using val_multiply_zero_64 unfold_const64 
+   apply (metis bin_eval_int intval_mul.simps(12) is_IntVal32_def is_IntVal_def times_Value_def)
+          using val_multiply_zero_64 intval_mul.simps(2) unfold_const64 
+   apply (metis (no_types, opaque_lifting) Value.exhaust intval_mul.simps(12) intval_mul.simps(8) 
+          intval_mul.simps(9) mult.commute mult_zero_left) 
+          using val_multiply_zero_64 bin_multiply_zero intval_mul.simps(2) unfold_const64 
+                intval_mul.simps(12) 
+   apply (smt (verit, ccfv_SIG) Value.disc(8) Value.sel(2) intval_mul.simps(11) intval_mul.simps(8) 
+          is_ObjRef_def times_Value_def val_to_bool.elims(3) val_to_bool.simps(4) 
+          valid_value.simps(19) wf_bool.elims(2) wf_bool.elims(3))
+
+           using val_multiply_zero_64 bin_multiply_zero intval_mul.simps(2) unfold_const64 
+                intval_mul.simps(12) 
+           sorry
+
+(* Optimizations *)
+optimization opt_EliminateRedundantNegative: "-x * -y \<longmapsto> x * y"
+   apply unfold_optimization unfolding le_expr_def
+   apply simp_all
+   apply auto using val_eliminate_redundant_negative bin_eval.simps(2)
+  by (metis BinaryExpr intval_negate.simps(3) times_Value_def)
+
+
+optimization opt_MultiplyNeutral32: "x * ConstantExpr (IntVal32 1) \<longmapsto> x"
+   apply unfold_optimization unfolding le_expr_def
+   apply simp_all
+   apply auto using val_multiply_neutral_32 bin_eval.simps(2) 
+  by (smt (z3) Value.discI(1) Value.distinct(9) intval_mul.elims times_Value_def)
+
+
+optimization opt_MultiplyNeutral64: "x * ConstantExpr (IntVal64 1) \<longmapsto> x"
+   apply unfold_optimization unfolding le_expr_def
+   apply simp_all
+   apply auto using val_multiply_neutral_64 
+  by (metis Value.exhaust evaltree_not_undef intval_mul.simps(12) intval_mul.simps(13) 
+      intval_mul.simps(14) is_IntVal64_def times_Value_def) 
+
+optimization opt_MultiplyZero32: "x * ConstantExpr (IntVal32 0) \<longmapsto> ConstantExpr (IntVal32 0)"
+   apply unfold_optimization unfolding le_expr_def
+   apply simp_all
+   apply auto using val_multiply_zero_32 bin_eval.simps(2) intval_mul.simps(1)
+  by (metis Value.disc(2) Value.exhaust intval_mul.simps(3) intval_mul.simps(5) intval_mul.simps(8) 
+      intval_mul.simps(9) times_Value_def unfold_const32)
+
+(* Need to prove exp_multiply_zero_64 *)
+optimization opt_MultiplyZero64: "x * ConstantExpr (IntVal64 0) \<longmapsto> ConstantExpr (IntVal64 0)"
+   apply unfold_optimization unfolding le_expr_def using exp_multiply_zero_64 
+   apply simp+ 
+  done
+
+(* Size issue *)
+optimization opt_MultiplyNegative32: "x * - (ConstantExpr (IntVal32 1)) \<longmapsto> UnaryExpr UnaryNeg x"
+   apply unfold_optimization unfolding le_expr_def
+   apply simp_all 
+   apply auto using val_multiply_negative_32
+   apply (smt (z3) Value.discI(1) Value.distinct(9) intval_mul.elims intval_negate.simps(1) 
+      times_Value_def unary_eval.simps(2) unfold_unary)
+  sorry 
+
+optimization opt_MultiplyNegative64: "x * - (ConstantExpr (IntVal64 1)) \<longmapsto> UnaryExpr UnaryNeg x"
+   apply unfold_optimization unfolding le_expr_def
+   apply simp_all 
+   apply auto 
+  sorry
+
+
+end (* End of MulPhase *)
+
+end (* End of file *)
