Optimizations/Canonicalizations/NegatePhase.thy
@@ -1,0 +1,122 @@
+theory NegatePhase
+  imports
+    Common
+begin
+
+section \<open>Optimizations for Negate Nodes\<close>
+
+phase NegatePhase
+  terminating size
+begin
+
+(* Word level proofs *)
+lemma bin_negative_cancel:
+ "-1 * (-1 * ((x::('a::len) word))) = x"
+  by auto
+
+value "(2 :: 32 word) >>> (31 :: nat)"
+value "-((2 :: 32 word) >> (31 :: nat))"
+
+lemma bin_negative_shift32:
+  shows "-((x :: 32 word) >> (31 :: nat)) = x >>> (31 :: nat)"
+  sorry
+
+(* Value level proofs *)
+lemma val_negative_cancel:
+  assumes "e \<noteq> UndefVal \<and> intval_negate e \<noteq> UndefVal"
+  shows "val[-(-(e))] = val[e]"
+  by (metis (no_types, lifting) assms intval_negate.elims intval_negate.simps(1) 
+      intval_negate.simps(2) verit_minus_simplify(4))
+
+lemma val_distribute_sub:
+  assumes "x \<noteq> UndefVal \<and> y \<noteq> UndefVal"
+  shows "val[-(x-y)] = val[y-x]"
+  using assms apply (cases x; cases y; auto)
+  done
+
+(* Exp level proofs *)
+lemma exp_distribute_sub:
+  shows "exp[-(x-y)] \<ge> exp[y-x]"
+   apply (cases x; cases y; auto) using unfold_binary val_distribute_sub 
+   apply auto[1]
+   apply (metis BinaryExpr UnaryExpr bin_eval.simps(3) val_distribute_sub) 
+          using bin_eval.simps(3) val_distribute_sub apply auto[1]
+   apply (metis BinaryExpr ParameterExpr UnaryExpr bin_eval.simps(3) intval_sub.simps(10) 
+          val_distribute_sub)
+   apply (metis BinaryExpr LeafExpr UnaryExpr bin_eval.simps(3) intval_sub.simps(10) 
+          val_distribute_sub)
+   apply (metis BinaryExpr ConstantExpr UnaryExpr bin_eval.simps(3) evaltree_not_undef 
+          val_distribute_sub)
+   apply (metis BinaryExpr UnaryExpr bin_eval.simps(3) val_distribute_sub)
+   apply (metis BinaryExpr bin_eval.simps(3) val_distribute_sub) using val_distribute_sub 
+   apply auto[1]
+   apply (metis BinaryExpr ParameterExpr bin_eval.simps(3) evaltree_not_undef val_distribute_sub)
+   apply (metis BinaryExpr LeafExpr bin_eval.simps(3) val_distribute_sub valid_value.simps(4))
+   apply (metis BinaryExpr ConstantExpr bin_eval.simps(3) evaltree_not_undef val_distribute_sub)
+          using unfold_binary val_distribute_sub apply auto[1]
+          using val_distribute_sub apply auto[1]
+          using unfold_binary val_distribute_sub apply auto[1]
+   apply (smt (verit, best) ConditionalExpr ParameterExpr bin_eval.simps(3) intval_sub.simps(10) 
+          unfold_binary val_distribute_sub)
+   apply (smt (verit, ccfv_SIG) BinaryExpr ConditionalExpr LeafExpr bin_eval.simps(3) 
+          intval_sub.simps(10) val_distribute_sub)
+   apply (smt (verit, ccfv_SIG) ConditionalExpr ConstantExpr bin_eval.simps(3) intval_sub.simps(10) 
+          unfold_binary val_distribute_sub)
+   apply (metis BinaryExpr ParameterExpr UnaryExpr bin_eval.simps(3) intval_sub.simps(3) 
+          val_distribute_sub)
+   apply (metis BinaryExpr ParameterExpr bin_eval.simps(3) evaltree_not_undef val_distribute_sub)
+   apply (smt (verit, ccfv_SIG) BinaryExpr ConditionalExpr ParameterExpr bin_eval.simps(3) 
+          evaltree_not_undef val_distribute_sub)
+   apply (metis BinaryExpr ParameterExpr bin_eval.simps(3) evaltree_not_undef val_distribute_sub)
+   apply (metis LeafExpr ParameterExpr bin_eval.simps(3) evaltree_not_undef unfold_binary 
+          val_distribute_sub)
+   apply (metis ConstantExpr ParameterExpr bin_eval.simps(3) unfold_binary val_distribute_sub 
+          valid_value.simps(4))
+   apply (metis BinaryExpr LeafExpr UnaryExpr bin_eval.simps(3) intval_sub.simps(3) 
+          val_distribute_sub)
+   apply (metis BinaryExpr LeafExpr bin_eval.simps(3) val_distribute_sub valid_value.simps(4))
+   apply (smt (verit, ccfv_SIG) ConditionalExpr LeafExpr bin_eval.simps(3) intval_sub.simps(3) 
+          unfold_binary val_distribute_sub)
+   apply (metis LeafExpr ParameterExpr bin_eval.simps(3) evaltree_not_undef unfold_binary 
+          val_distribute_sub)
+   apply (metis LeafExpr bin_eval.simps(3) intval_sub.simps(10) intval_sub.simps(3) unfold_binary 
+          val_distribute_sub)
+   apply (metis BinaryExpr ConstantExpr LeafExpr bin_eval.simps(3) evaltree_not_undef 
+          val_distribute_sub)
+   apply (metis BinaryExpr ConstantExpr UnaryExpr bin_eval.simps(3) evaltree_not_undef 
+          val_distribute_sub)
+   apply (metis BinaryExpr ConstantExpr bin_eval.simps(3) evaltree_not_undef val_distribute_sub)
+   apply (smt (verit, ccfv_SIG) BinaryExpr ConditionalExpr ConstantExpr bin_eval.simps(3) 
+          evaltree_not_undef val_distribute_sub)
+   apply (metis BinaryExpr ConstantExpr ParameterExpr bin_eval.simps(3) intval_sub.simps(10) 
+          intval_sub.simps(3) val_distribute_sub)
+   apply (metis BinaryExpr ConstantExpr LeafExpr bin_eval.simps(3) evaltree_not_undef 
+          val_distribute_sub)
+   apply (metis BinaryExpr ConstantExpr bin_eval.simps(3) evaltree_not_undef val_distribute_sub) 
+  done
+
+(* Optimisations *)
+optimization negate_cancel: "-(-(e)) \<longmapsto> e"
+   apply simp_all
+  by (metis intval_negate.simps(3) unary_eval.simps(2) unfold_unary val_negative_cancel)
+
+
+(* FloatStamp condition is omitted. Not 100% sure. *)
+optimization distribute_sub: "-(x - y) \<longmapsto> (y - x)" 
+   apply simp_all 
+   apply auto
+   apply (simp add: BinaryExpr evaltree_not_undef val_distribute_sub)
+  done
+
+
+(* Bits: 64, 32, 16, 8, 1 *)
+(* 32-bit proof *)
+optimization negative_shift_32: "-(BinaryExpr BinRightShift x (const (IntVal32 31))) \<longmapsto> 
+                                   BinaryExpr BinURightShift x (const (IntVal32 31))"
+   apply simp_all
+  sorry
+
+
+end (* End of NegatePhase *)
+
+end (* End of file *)
