Optimizations/Canonicalizations/NotPhase.thy
@@ -1,0 +1,39 @@
+theory NotPhase
+  imports
+    Common
+begin
+
+section \<open>Optimizations for Not Nodes\<close>
+
+phase NotPhase
+  terminating size
+begin
+
+(* Word level proofs *)
+lemma bin_not_cancel:
+ "bin[\<not>(\<not>(e))] = bin[e]"
+  by auto
+
+(* Value level proofs *)
+lemma val_not_cancel:
+  assumes "e \<noteq> UndefVal \<and> (intval_not e) \<noteq> UndefVal \<and> intval_not (intval_not e) \<noteq> UndefVal"
+  shows "intval_not (intval_not e) = e"
+  using bin_not_cancel
+  by (metis (no_types, lifting) assms intval_not.elims intval_not.simps(1) intval_not.simps(2))
+
+(* Expr level proofs *)
+lemma exp_not_cancel:
+  shows "UnaryExpr UnaryNot (UnaryExpr UnaryNot a) \<ge> exp[a]"
+   apply simp using val_not_cancel
+  by (metis UnaryExprE intval_not.simps(3) unary_eval.simps(3))
+
+(* Optimisations *)
+optimization not_cancel: "UnaryExpr UnaryNot (UnaryExpr UnaryNot a) \<longmapsto> a"
+   apply unfold_optimization
+   apply simp_all
+   apply auto
+ by (metis intval_not.simps(3) val_not_cancel)
+
+end (* End of NotPhase *)
+
+end (* End of file *)
