Optimizations/Canonicalizations/OrPhase.thy
@@ -1,0 +1,111 @@
+theory OrPhase
+  imports
+    Common
+    NewAnd (* Allows access to mask operations *)
+begin
+
+section \<open>Optimizations for Or Nodes\<close>
+
+phase OrPhase
+  terminating size
+begin
+
+(* Word level proofs *)
+lemma bin_or_equal:
+  "bin[x | x] = bin[x]"
+  by simp
+
+lemma bin_shift_const_right_helper:
+ "x | y = y | x"
+  by simp
+
+lemma bin_or_not_operands:
+ "(~x | ~y) = (~(x & y))"
+  by simp
+
+(* Value level proofs *)
+lemma val_or_equal:
+  assumes "x \<noteq> UndefVal \<and> ((intval_or x x) \<noteq> UndefVal)"
+  shows "val[x | x] = val[x]"
+   apply (cases x; auto) using bin_or_equal assms 
+   apply auto+ 
+  done
+
+lemma val_elim_redundant_false:
+  assumes "x \<noteq> UndefVal \<and> (intval_or x (bool_to_val False)) \<noteq> UndefVal"
+  shows "val[x | false] = val[x]"
+   using assms apply (cases x) 
+  by simp+
+
+lemma val_shift_const_right_helper:
+   "val[x | y] = val[y | x]"
+   apply (cases x; cases y; auto)
+   apply (simp add: or.commute)+
+  done
+
+lemma val_or_not_operands:
+ "intval_or (intval_not x) (intval_not y) = intval_not (intval_and x y)"
+  apply (cases x; cases y; auto)
+  done
+
+(* Expr level proofs *)
+lemma exp_or_equal:
+  "exp[x | x] \<ge> exp[x]"
+   apply simp using val_or_equal
+  by (metis bin_eval.simps(5) evalDet evaltree_not_undef unfold_binary)
+
+lemma exp_elim_redundant_false:
+ "exp[x | false] \<ge> exp[x]"
+   apply simp using val_elim_redundant_false 
+   apply (cases x)
+   apply (metis BinaryExprE bin_eval.simps(5) bool_to_val.simps(2) evaltree_not_undef 
+          unfold_const32)+
+  done
+  
+(* Optimizations *)
+optimization or_equal: "x | x \<longmapsto> x"
+   apply unfold_optimization
+   apply simp_all
+  by (meson exp_or_equal le_expr_def)
+
+
+optimization OrShiftConstantRight: "((const x) | y) \<longmapsto> y | (const x) when \<not>(is_ConstantExpr y)"
+   apply unfold_optimization unfolding le_expr_def using val_shift_const_right_helper 
+   apply auto[1] using size_non_const
+   apply simp
+  done
+
+optimization elim_redundant_false: "x | false \<longmapsto> x"
+   apply unfold_optimization
+   apply simp_all
+  by (meson exp_elim_redundant_false le_expr_def)
+
+
+(* Broke after changes to size function. 15/07 *)
+optimization or_not_operands: "(UnaryExpr UnaryNot x | UnaryExpr UnaryNot y) \<longmapsto> 
+                                UnaryExpr UnaryNot (x & y)"
+   apply unfold_optimization
+   apply simp_all
+   apply auto using val_or_not_operands
+   apply (metis bin_eval.simps(4) intval_not.simps(3) unary_eval.simps(3) unfold_binary 
+          unfold_unary)
+  sorry
+
+optimization or_left_fall_through: "(x | y) \<longmapsto> x
+                                when (((and (not (IRExpr_down x)) (IRExpr_up y)) = 0))"
+   apply unfold_optimization 
+   apply simp_all 
+   apply auto
+   apply (simp add: IRExpr_down_def IRExpr_up_def) 
+  done
+
+optimization or_right_fall_through: "(x | y) \<longmapsto> y
+                                when (((and (not (IRExpr_down y)) (IRExpr_up x)) = 0))"
+   apply unfold_optimization
+   apply (meson exp_or_commute or_left_fall_through(1) order.trans rewrite_preservation.simps(2))
+   apply simp_all
+  done
+
+end (* End of OrPhase *)
+
+end (* End of file *)
