Optimizations/Canonicalizations/SubPhase.thy
@@ -1,0 +1,264 @@
+theory SubPhase
+  imports
+    Common
+begin
+
+section \<open>Optimizations for Sub Nodes\<close>
+
+phase SubPhase
+  terminating size
+begin
+
+(* Word level proofs *)
+
+lemma bin_sub_after_right_add:
+  shows "((x::('a::len) word) + (y::('a::len) word)) - y = x"
+  by simp
+
+lemma sub_self_is_zero:
+  shows "(x::('a::len) word) - x = 0"
+  by simp
+
+lemma bin_sub_then_left_add:
+  shows "(x::('a::len) word) - (x + (y::('a::len) word)) = -y"
+  by simp
+
+lemma bin_sub_then_left_sub:
+  shows "(x::('a::len) word) - (x - (y::('a::len) word)) = y"
+  by simp
+
+lemma bin_subtract_zero:
+  shows "(x :: 'a::len word) - (0 :: 'a::len word) = x"
+  by simp
+
+lemma bin_sub_negative_value:
+ "(x :: ('a::len) word) - (-(y :: ('a::len) word)) = x + y"
+  by simp
+
+lemma bin_sub_self_is_zero:
+ "(x :: ('a::len) word) - x = 0"
+  by simp
+
+lemma bin_sub_negative_const:
+"(x :: 'a::len word) - (-(y :: 'a::len word)) = x + y"
+  by simp
+
+(* Value level proofs *)
+
+lemma val_sub_after_right_add_2:
+  assumes "y \<noteq> UndefVal \<and> x \<noteq> UndefVal \<and> ((x + y) - y \<noteq> UndefVal)"
+  shows "val[(x + y) - (y)] = val[x]"
+  using bin_sub_after_right_add 
+  using assms apply (cases x; cases y; auto) apply (simp add: minus_Value_def plus_Value_def)
+  by (simp add: minus_Value_def plus_Value_def)+
+
+lemma val_sub_after_left_sub:
+  assumes "y \<noteq> UndefVal \<and> x \<noteq> UndefVal \<and> ((x - y) - x \<noteq> UndefVal)"
+  shows "val[(x - y) - x] = val[-y]"
+  using assms apply (cases x; cases y; auto) apply (simp add: minus_Value_def)
+    by (simp add: minus_Value_def)+
+
+lemma val_sub_then_left_sub:
+  assumes "y \<noteq> UndefVal \<and> x \<noteq> UndefVal \<and> (x - (x - y) \<noteq> UndefVal)"
+  shows "val[x - (x - y)] = val[y]"
+  using assms apply (cases x; cases y; auto) apply (simp add: minus_Value_def)
+    by (simp add: minus_Value_def)+
+
+lemma val_subtract_zero:
+  assumes "x \<noteq> UndefVal \<and> intval_sub x (IntVal32 0) \<noteq> UndefVal "
+  shows "intval_sub x (IntVal32 0) = val[x]"
+  using assms by (induction x; simp)
+
+lemma val_zero_subtract_value:
+  assumes "x \<noteq> UndefVal \<and> intval_sub (IntVal32 0) x \<noteq> UndefVal "
+  shows "intval_sub (IntVal32 0) x = val[-x]"
+  using assms by (induction x; simp)
+
+lemma val_zero_subtract_value_64:
+  assumes "x \<noteq> UndefVal \<and> intval_sub (IntVal64 0) x \<noteq> UndefVal "
+  shows "intval_sub (IntVal64 0) x = val[-x]"
+  using assms by (induction x; simp)
+
+lemma val_sub_then_left_add:
+  assumes "y \<noteq> UndefVal \<and> x \<noteq> UndefVal \<and> (x - (x + y) \<noteq> UndefVal)"
+  shows "val[x - (x + y)] = val[-y]"
+  using assms apply (cases x; cases y; auto) apply (simp add: minus_Value_def plus_Value_def)
+  by (simp add: minus_Value_def plus_Value_def)+
+
+lemma val_sub_negative_value:
+  assumes "y \<noteq> UndefVal \<and> x \<noteq> UndefVal \<and> (x - (intval_negate y) \<noteq> UndefVal)"
+  shows "val[x - (-y)] = val[x + y]"
+  using assms apply (cases x; cases y)
+  by (simp add: minus_Value_def plus_Value_def)+
+
+(* 32 *)
+lemma val_sub_self_is_zero:
+  assumes "is_IntVal32 x \<and> x \<noteq> UndefVal \<and> x - x \<noteq> UndefVal"
+  shows "val[x - x] = IntVal32 0"
+  using assms apply (cases x; auto)
+  done
+
+(* 64 *)
+lemma val_sub_self_is_zero_2:
+  assumes "is_IntVal64 x \<and> x \<noteq> UndefVal \<and> x - x \<noteq> UndefVal"
+  shows "val[x - x] = IntVal64 0"
+  using assms apply (cases x; auto)
+  done
+
+lemma val_sub_negative_const:
+  assumes "is_IntVal32 y \<or> is_IntVal64 y \<and> y \<noteq> UndefVal \<and> x \<noteq> UndefVal \<and> 
+           x - (intval_negate y) \<noteq> UndefVal"
+  shows "x - (intval_negate y) = x + y"
+  using assms apply (cases x; cases y; auto)
+    by (simp add: minus_Value_def plus_Value_def)+
+
+
+(* Expression level proofs *)
+
+lemma exp_sub_after_right_add:
+  shows "exp[(x+y)-y] \<ge> exp[x]"
+  apply simp
+  apply auto
+  by (metis evalDet evaltree_not_undef minus_Value_def plus_Value_def val_sub_after_right_add_2)
+
+lemma exp_sub_negative_value:
+ "exp[x - (-y)] \<ge> exp[x + y]"
+  apply simp using val_sub_negative_value
+  by (smt (verit) bin_eval.simps(1) bin_eval.simps(3) evaltree_not_undef minus_Value_def 
+      unary_eval.simps(2) unfold_binary unfold_unary)
+
+(* Optimizations *)
+optimization sub_after_right_add: "((x + y) - y) \<longmapsto>  x"
+   apply unfold_optimization
+   apply simp_all
+   apply auto
+  by (metis evalDet evaltree_not_undef minus_Value_def plus_Value_def val_sub_after_right_add_2)
+
+optimization sub_after_left_add: "((x + y) - x) \<longmapsto>  y"
+   apply unfold_optimization
+   apply simp_all
+   apply auto
+  by (metis add.commute evalDet intval_add.simps(10) minus_Value_def plus_Value_def 
+      val_sub_after_right_add_2)
+
+optimization sub_after_left_sub: "((x - y) - x) \<longmapsto>  -y"
+   apply unfold_optimization
+   apply simp_all
+   apply auto
+   apply (metis evalDet intval_sub.simps(10) minus_Value_def unary_eval.simps(2) unfold_unary 
+          val_sub_after_left_sub)
+  done 
+
+optimization sub_then_left_add: "(x - (x + y)) \<longmapsto> -y"
+   apply unfold_optimization
+   apply simp_all
+   apply auto
+   apply (metis UnaryExpr evalDet evaltree_not_undef minus_Value_def plus_Value_def 
+          unary_eval.simps(2) val_sub_then_left_add)
+  done
+
+optimization sub_then_right_add: "(y - (x + y)) \<longmapsto> -x"
+   apply unfold_optimization
+   apply simp_all
+   apply auto
+   apply (metis UnaryExpr add.commute evalDet evaltree_not_undef minus_Value_def plus_Value_def 
+          unary_eval.simps(2) val_sub_then_left_add)
+  done
+
+
+optimization sub_then_left_sub: "(x - (x - y)) \<longmapsto> y"
+   apply unfold_optimization
+   apply simp_all
+   apply auto
+  by (metis evalDet evaltree_not_undef minus_Value_def val_sub_then_left_sub)
+
+
+(* 32-bit *)
+optimization subtract_zero: "(x - (const IntVal32 0)) \<longmapsto> x"
+   apply unfold_optimization
+   apply simp_all
+   apply auto
+  by (metis evaltree_not_undef val_subtract_zero)
+
+(* 64-bit *)
+optimization subtract_zero_64: "(x - (const IntVal64 0)) \<longmapsto> x"
+   apply unfold_optimization
+   apply simp_all
+   apply auto 
+   apply (smt (z3) Value.sel(2) diff_zero intval_sub.elims intval_sub.simps(12)) 
+  done
+
+optimization sub_negative_value: "(x - (-y)) \<longmapsto> x + y"
+   apply unfold_optimization
+   apply simp_all using exp_sub_negative_value 
+   apply auto
+  done
+
+(* Ln 146 rewrite, 32-bit *)
+optimization sub_negative_const2: "(x - (const (intval_negate (IntVal32 y)))) \<longmapsto> 
+                                    x + (const (IntVal32 y)) 
+                                    when (y < 0)"
+   apply unfold_optimization
+   apply auto
+  done 
+
+(* Ln 146 rewrite, 64-bit *)
+optimization sub_negative_const2_64: "(x - (const (intval_negate (IntVal64 y)))) \<longmapsto> 
+                                       x + (const (IntVal64 y)) 
+                                       when (y < 0)"
+   apply unfold_optimization
+   apply auto
+  done 
+
+(* 32-bit *)
+optimization zero_sub_value: "((const IntVal32 0) - x) \<longmapsto> -x"
+   apply unfold_optimization unfolding size.simps
+   apply simp_all
+   apply auto
+   apply (metis UnaryExpr intval_sub.simps(10) unary_eval.simps(2) val_zero_subtract_value)
+  done
+
+(* 64-bit *)
+optimization zero_sub_value_64: "((const IntVal64 0) - x) \<longmapsto> -x"
+   apply unfold_optimization unfolding size.simps
+   apply simp_all
+   apply auto 
+   apply (metis UnaryExpr intval_sub.simps(10) unary_eval.simps(2) val_zero_subtract_value_64)
+  done
+
+(* wf_stamp definition borrowed from ConditionalPhase *)
+definition wf_stamp :: "IRExpr \<Rightarrow> bool" where
+  "wf_stamp e = (\<forall>m p v. ([m, p] \<turnstile> e \<mapsto> v) \<longrightarrow> valid_value v (stamp_expr e))"
+
+(* 32-bit *)
+optimization opt_sub_self_is_zero32: "(x - x) \<longmapsto> const IntVal32 0 when 
+                      (wf_stamp x \<and> stamp_expr x = default_stamp)"
+   apply unfold_optimization 
+   apply simp_all 
+   apply auto defer
+   apply (metis less_1_mult less_one linorder_neqE_nat mult.commute mult_1 numeral_1_eq_Suc_0 
+          one_eq_numeral_iff one_less_numeral_iff semiring_norm(77) size_pos 
+          zero_less_iff_neq_zero)
+   apply (metis (no_types, lifting) Value.distinct(1) a0a_helper add.inverse_neutral evalDet 
+         intval_negate.simps(1) intval_sub.simps(10) minus_Value_def plus_Value_def unfold_const32 
+         val_sub_then_left_add wf_stamp_def)
+  done
+
+(* 64-bit *)
+(*
+optimization opt_sub_self_is_zero64: "(x - x) \<longmapsto> const IntVal64 0 when 
+                      (wf_stamp x \<and> stamp_expr x = (unrestricted_stamp (IntegerStamp 64 0 0)))"
+   apply unfold_optimization 
+   apply simp_all 
+   apply auto defer
+   apply (metis less_1_mult less_one linorder_neqE_nat mult.commute mult_1 numeral_1_eq_Suc_0 
+          one_eq_numeral_iff one_less_numeral_iff semiring_norm(77) size_pos 
+          zero_less_iff_neq_zero) using val_sub_self_is_zero_2 wf_stamp_def
+   apply (metis (no_types, lifting) evalDet intval_sub.simps(10) is_IntVal64_def minus_Value_def 
+          unfold_const64 valid_int64)  
+  done
+*)
+
+end (* End of SubPhase *)
+
+end (* End of file *)
